Parser/Error.lean
@@ -29,7 +29,8 @@ instance (σ τ) [Parser.Stream σ τ] : Parser.Error (Basic σ τ) σ τ where
   unexpected p t := (p, t)
   addMessage e _ _ := e
 
-instance (σ τ) [Repr τ] [Parser.Stream σ τ] [Repr (Parser.Stream.Position σ)] : ToString (Basic σ τ) where
+instance (σ τ) [Repr τ] [Parser.Stream σ τ] [Repr (Parser.Stream.Position σ)] :
+  ToString (Basic σ τ) where
   toString
     | (pos, some tok) => s!"unexpected input {repr tok} at {repr pos}"
     | (pos, none) => s!"unexpected input at {repr pos}"
@@ -42,7 +43,8 @@ inductive Simple (σ τ) [Parser.Stream σ τ]
   | addMessage : Simple σ τ → Stream.Position σ → String → Simple σ τ
 
 -- The derive handler for `Repr` fails, this is a workaround.
-private def Simple.reprPrec {σ τ} [Parser.Stream σ τ] [Repr τ] [Repr (Stream.Position σ)] : Simple σ τ → Nat → Std.Format
+private def Simple.reprPrec {σ τ} [Parser.Stream σ τ] [Repr τ] [Repr (Stream.Position σ)] :
+  Simple σ τ → Nat → Std.Format
   | unexpected pos a, prec =>
     Repr.addAppParen
       (Std.Format.group
@@ -69,12 +71,14 @@ private def Simple.reprPrec {σ τ} [Parser.Stream σ τ] [Repr τ] [Repr (Strea
 instance (σ τ) [Parser.Stream σ τ] [Repr τ] [Repr (Stream.Position σ)] : Repr (Simple σ τ) where
   reprPrec := Simple.reprPrec
 
-private def Simple.toString {σ τ} [Repr τ] [Parser.Stream σ τ] [Repr (Parser.Stream.Position σ)] : Simple σ τ → String
+private def Simple.toString {σ τ} [Repr τ] [Parser.Stream σ τ] [Repr (Parser.Stream.Position σ)] :
+  Simple σ τ → String
   | unexpected pos (some tok) => s!"unexpected token {repr tok} at {repr pos}"
   | unexpected pos none => s!"unexpected token at {repr pos}"
   | addMessage e pos msg => Simple.toString e ++ s!"; {msg} at {repr pos}"
 
-instance (σ τ) [Repr τ] [Parser.Stream σ τ] [Repr (Parser.Stream.Position σ)] : ToString (Simple σ τ) where
+instance (σ τ) [Repr τ] [Parser.Stream σ τ] [Repr (Parser.Stream.Position σ)] :
+  ToString (Simple σ τ) where
   toString := Simple.toString
 
 instance (σ τ) [Parser.Stream σ τ] : Parser.Error (Simple σ τ) σ τ where
